ImplModelSync progress

disk-betree/ImplModelSync.i.dfy
@@ -57,7 +57,7 @@ module ImplModelSync {
     )
   }
 
-  function {:fuel JoinBucketList,0} fixBigNode(k: Constants, s: Variables, io: IO, ref: BT.G.Reference, parentref: BT.G.Reference)
+  function {:fuel JoinBucketList,0} {:opaque} fixBigNode(k: Constants, s: Variables, io: IO, ref: BT.G.Reference, parentref: BT.G.Reference)
   : (Variables, IO)
   requires Inv(k, s)
   requires s.Ready?
@@ -124,6 +124,8 @@ module ImplModelSync {
     && WFVars(s')
     && M.Next(Ik(k), IVars(s), IVars(s'), UI.NoOp, diskOp(io'))
   {
+    reveal_fixBigNode();
+
     var (s', io') := fixBigNode(k, s, io, ref, parentref);
 
     if (ref !in s.cache) {
@@ -176,257 +178,244 @@ module ImplModelSync {
     }
   }
 
-  /*
-  method AssignRefToLBA(table: MutIndirectionTable, ref: Reference, loc: BC.Location)
-  requires table.Inv()
-  ensures table.Inv()
-  ensures IIndirectionTable(table) == old(BC.assignRefToLocation(IIndirectionTable(table), ref, loc))
+  function {:opaque} AssignRefToLoc(table: IndirectionTable, ref: Reference, loc: BC.Location) : IndirectionTable
   {
-    var locGraph := table.Remove(ref);
-    if locGraph.Some? {
-      var (_, graph) := locGraph.value;
-      assume table.Count as nat < 0x10000000000000000 / 8;
-      var _ := table.Insert(ref, (Some(loc), graph));
-    }
-    assert IIndirectionTable(table) ==
-        old(BC.assignRefToLocation(IIndirectionTable(table), ref, loc));
+    if (ref in table) then (
+      table[ref := (Some(loc), table[ref].1)]
+    ) else (
+      table
+    )
   }
 
-  method FindUncappedNodeInCache(s: Variables) returns (ref: Option<Reference>)
+  lemma AssignRefToLocCorrect(table: IndirectionTable, ref: Reference, loc: BC.Location)
+  ensures var table' := AssignRefToLoc(table, ref, loc);
+    IIndirectionTable(table') == BC.assignRefToLocation(IIndirectionTable(table), ref, loc)
+  {
+    reveal_AssignRefToLoc();
+  }
+
+  function {:opaque} FindUncappedNodeInCache(s: Variables) : (ref: Option<Reference>)
   requires WFVars(s)
   requires s.Ready?
-  ensures ref.Some? ==> ref.value in IIndirectionTable(s.ephemeralIndirectionTable).graph
-  ensures ref.Some? ==> ref.value in s.cache && !Marshalling.CappedNode(s.cache[ref.value])
-  ensures ref.None? ==> forall r | r in IIndirectionTable(s.ephemeralIndirectionTable).graph :: r !in s.cache || Marshalling.CappedNode(s.cache[r])
-  {
-    // TODO once we have an lba freelist, rewrite this to avoid extracting a `map` from `s.ephemeralIndirectionTable`
-    var ephemeralTable := s.ephemeralIndirectionTable.ToMap();
-    var ephemeralRefs := SetToSeq(ephemeralTable.Keys);
 
-    assume |ephemeralRefs| < 0x1_0000_0000_0000_0000;
+  lemma FindUncappedNodeInCacheCorrect(s: Variables)
+  requires WFVars(s)
+  requires s.Ready?
+  ensures var ref := FindUncappedNodeInCache(s);
+    && (ref.Some? ==> ref.value in s.ephemeralIndirectionTable)
+    && (ref.Some? ==> ref.value in s.cache && !IMM.CappedNode(s.cache[ref.value]))
+    && (ref.None? ==> forall r | r in s.ephemeralIndirectionTable :: r !in s.cache || IMM.CappedNode(s.cache[r]))
 
-    var i: uint64 := 0;
-    while i as int < |ephemeralRefs|
-    invariant i as int <= |ephemeralRefs|
-    invariant forall k : nat | k < i as nat :: (
-        && ephemeralRefs[k] in IIndirectionTable(s.ephemeralIndirectionTable).graph
-        && (ephemeralRefs[k] !in s.cache || Marshalling.CappedNode(s.cache[ephemeralRefs[k]])))
-    {
-      var ref := ephemeralRefs[i];
-      if ref in s.cache && !Marshalling.CappedNode(s.cache[ref]) {
-        return Some(ref);
-      }
-      i := i + 1;
-    }
-    assert forall r | r in IIndirectionTable(s.ephemeralIndirectionTable).graph :: r !in s.cache || Marshalling.CappedNode(s.cache[r]);
-    return None;
-  }
-
-  method FindRefInFrozenWithNoLba(s: Variables) returns (ref: Option<Reference>)
+  function {:opaque} FindRefInFrozenWithNoLoc(s: Variables) : (ref: Option<Reference>)
   requires WFVars(s)
   requires s.Ready?
   requires s.frozenIndirectionTable.Some?
-  ensures ref.Some? ==> ref.value in IIndirectionTable(s.frozenIndirectionTable.value).graph 
-  ensures ref.Some? ==> ref.value !in IIndirectionTable(s.frozenIndirectionTable.value).locs
-  ensures ref.None? ==> forall r | r in IIndirectionTable(s.frozenIndirectionTable.value).graph
-      :: r in IIndirectionTable(s.frozenIndirectionTable.value).locs
-  {
-    // TODO once we have an lba freelist, rewrite this to avoid extracting a `map` from `s.ephemeralIndirectionTable`
-    var frozenTable := s.frozenIndirectionTable.value.ToMap();
-    var frozenRefs := SetToSeq(frozenTable.Keys);
 
-    assume |frozenRefs| < 0x1_0000_0000_0000_0000;
-
-    var i: uint64 := 0;
-    while i as int < |frozenRefs|
-    invariant i as int <= |frozenRefs|
-    invariant forall k : nat | k < i as nat :: (
-        && frozenRefs[k] in IIndirectionTable(s.frozenIndirectionTable.value).graph
-        && frozenRefs[k] in IIndirectionTable(s.frozenIndirectionTable.value).locs)
-    {
-      var ref := frozenRefs[i];
-      var lbaGraph := s.frozenIndirectionTable.value.Get(ref);
-      assert lbaGraph.Some?;
-      var (lba, _) := lbaGraph.value;
-      if lba.None? {
-        return Some(ref);
-      }
-      i := i + 1;
-    }
-    assert forall r | r in IIndirectionTable(s.frozenIndirectionTable.value).graph
-        :: r in IIndirectionTable(s.frozenIndirectionTable.value).locs;
-    return None;
-  }
-
-  method FindRefNotPointingToRefInEphemeral(s: Variables, ref: Reference) returns (result: Reference)
+  lemma FindRefInFrozenWithNoLocCorrect(s: Variables)
   requires WFVars(s)
   requires s.Ready?
-  requires exists r :: r in IIndirectionTable(s.ephemeralIndirectionTable).graph && 
-      ref in IIndirectionTable(s.ephemeralIndirectionTable).graph[r]
-  ensures result in IIndirectionTable(s.ephemeralIndirectionTable).graph && 
-      ref in IIndirectionTable(s.ephemeralIndirectionTable).graph[result]
-  {
-    assert s.ephemeralIndirectionTable.Inv();
-    var ephemeralTable := s.ephemeralIndirectionTable.ToMap();
+  requires s.frozenIndirectionTable.Some?
+  ensures var ref := FindRefInFrozenWithNoLoc(s);
+    && (ref.Some? ==> ref.value in s.frozenIndirectionTable.value)
+    && (ref.Some? ==> s.frozenIndirectionTable.value[ref.value].0.None?)
+    && (ref.None? ==> forall r | r in s.frozenIndirectionTable.value
+        :: s.frozenIndirectionTable.value[r].0.Some?)
 
-    var ephemeralRefs := SetToSeq(ephemeralTable.Keys);
-    assert forall k | k in ephemeralRefs :: k in ephemeralTable;
-
-    assert forall k | k in ephemeralRefs :: k in IIndirectionTable(s.ephemeralIndirectionTable).graph; // TODO
-
-    // TODO how do we deal with this?
-    assume |ephemeralRefs| < 0x1_0000_0000_0000_0000;
-
-    var i: uint64 := 0;
-    while i as nat < |ephemeralRefs|
-    invariant i as nat <= |ephemeralRefs|
-    invariant forall k : nat | k < i as nat :: (
-        || ephemeralRefs[k] !in IIndirectionTable(s.ephemeralIndirectionTable).graph
-        || ref !in IIndirectionTable(s.ephemeralIndirectionTable).graph[ephemeralRefs[k]])
-    {
-      var eRef := ephemeralRefs[i];
-      assert eRef in IIndirectionTable(s.ephemeralIndirectionTable).graph;
-
-      var lbaGraph := s.ephemeralIndirectionTable.Get(eRef);
-      assert lbaGraph.Some?;
-
-      var (_, graph) := lbaGraph.value;
-      if ref in graph {
-        assert eRef in IIndirectionTable(s.ephemeralIndirectionTable).graph && 
-            ref in IIndirectionTable(s.ephemeralIndirectionTable).graph[eRef];
-        return eRef;
-      }
-
-      i := i + 1;
-    }
-    assert false;
-  }
-
-  method {:fuel BC.GraphClosed,0} {:fueld BC.CacheConsistentWithSuccessors,0}
-  syncNotFrozen(k: Constants, s: Variables, io: IO)
-  returns (s': Variables)
-  requires io.initialized()
-  modifies io
+  function {:opaque} FindParentRef(s: Variables, ref: Reference) : (parentref: Reference)
   requires WFVars(s)
-  requires BBC.Inv(k, IVars(s))
+  requires s.Ready?
+
+  lemma FindParentRefCorrect(s: Variables, ref: Reference)
+  requires WFVars(s)
+  requires s.Ready?
+  ensures var parentref := FindParentRef(s, ref);
+    && parentref in IIndirectionTable(s.ephemeralIndirectionTable).graph
+    && ref in IIndirectionTable(s.ephemeralIndirectionTable).graph[parentref]
+
+  function {:fuel BC.GraphClosed,0} {:fuel BC.CacheConsistentWithSuccessors,0}
+  syncNotFrozen(k: Constants, s: Variables, io: IO)
+  : (res: (Variables, IO))
+  requires io.IOInit?
+  requires Inv(k, s)
   requires s.Ready?
   requires s.outstandingIndirectionTableWrite.None?
-  requires s.rootBucket == TTT.EmptyTree
+  requires s.rootBucket == map[]
   requires s.frozenIndirectionTable.None?
-  ensures WFVars(s')
-  ensures ImplADM.Next(Ik(k), IVars(s), IVars(s'), UI.NoOp, io.diskOp())
   {
-    var ephemeralTable := s.ephemeralIndirectionTable.ToMap();
+    var ephemeralTable := s.ephemeralIndirectionTable;
     var ephemeralGraph := map k | k in ephemeralTable :: ephemeralTable[k].1;
+
     var foundDeallocable := FindDeallocable(s);
+    FindDeallocableCorrect(s);
+
+    if foundDeallocable.Some? then (
+      Dealloc(k, s, io, foundDeallocable.value)
+    ) else (
+      var foundUncapped := FindUncappedNodeInCache(s);
+      FindUncappedNodeInCacheCorrect(s);
+      if foundUncapped.Some? then (
+        var ref := foundUncapped.value;
+        if (ref == BT.G.Root()) then (
+          fixBigRoot(k, s, io)
+        ) else (
+          var r := FindParentRef(s, ref);
+          FindParentRefCorrect(s, ref);
+
+          fixBigNode(k, s, io, ref, r)
+        )
+      ) else (
+        var s' := s
+            .(frozenIndirectionTable := Some(s.ephemeralIndirectionTable))
+            .(syncReqs := BC.syncReqs3to2(s.syncReqs));
+        (s', io)
+      )
+    )
+  }
+
+  lemma {:fuel BC.GraphClosed,0} {:fuel BC.CacheConsistentWithSuccessors,0}
+  syncNotFrozenCorrect(k: Constants, s: Variables, io: IO)
+  requires io.IOInit?
+  requires Inv(k, s)
+  requires s.Ready?
+  requires s.outstandingIndirectionTableWrite.None?
+  requires s.rootBucket == map[]
+  requires s.frozenIndirectionTable.None?
+
+  ensures var (s', io') := syncNotFrozen(k, s, io);
+    && WFVars(s')
+    && M.Next(Ik(k), IVars(s), IVars(s'), UI.NoOp, diskOp(io'))
+  {
+    var (s', io') := syncNotFrozen(k, s, io);
+
+    var ephemeralTable := s.ephemeralIndirectionTable;
+    var ephemeralGraph := map k | k in ephemeralTable :: ephemeralTable[k].1;
+
+    var foundDeallocable := FindDeallocable(s);
+    FindDeallocableCorrect(s);
+
     if foundDeallocable.Some? {
-      s' := Dealloc(k, s, io, foundDeallocable.value);
+      DeallocCorrect(k, s, io, foundDeallocable.value);
       return;
     }
     var foundUncapped := FindUncappedNodeInCache(s);
+    FindUncappedNodeInCacheCorrect(s);
     if foundUncapped.Some? {
       var ref := foundUncapped.value;
       assert ref in IIndirectionTable(s.ephemeralIndirectionTable).graph;
-      assert ref in s.cache && !Marshalling.CappedNode(s.cache[foundUncapped.value]);
+      assert ref in s.cache && !IMM.CappedNode(s.cache[foundUncapped.value]);
       if (ref == BT.G.Root()) {
-        s' := fixBigRoot(k, s, io);
+        fixBigRootCorrect(k, s, io);
         return;
       } else {
-        assert !deallocable(s, ref);
-        assert !(forall r | r in IIndirectionTable(s.ephemeralIndirectionTable).graph ::
-            ref !in IIndirectionTable(s.ephemeralIndirectionTable).graph[r]);
-        assert !(forall r :: r in IIndirectionTable(s.ephemeralIndirectionTable).graph ==>
-            ref !in IIndirectionTable(s.ephemeralIndirectionTable).graph[r]);
-        assert (exists r :: !(r in IIndirectionTable(s.ephemeralIndirectionTable).graph ==>
-            ref !in IIndirectionTable(s.ephemeralIndirectionTable).graph[r]));
-        var r := FindRefNotPointingToRefInEphemeral(s, ref);
-        assert !(r in IIndirectionTable(s.ephemeralIndirectionTable).graph ==>
-            ref !in IIndirectionTable(s.ephemeralIndirectionTable).graph[r]);
-        s' := fixBigNode(k, s, io, ref, r);
+        var r := FindParentRef(s, ref);
+        FindParentRefCorrect(s, ref);
+        fixBigNodeCorrect(k, s, io, ref, r);
         return;
       }
     } else {
-      var clonedEphemeralIndirectionTable := s.ephemeralIndirectionTable.Clone();
-      assert IIndirectionTable(clonedEphemeralIndirectionTable) == IIndirectionTable(s.ephemeralIndirectionTable); // observe
-
-      s' := s
-          .(frozenIndirectionTable := Some(clonedEphemeralIndirectionTable))
-          .(syncReqs := BC.syncReqs3to2(s.syncReqs));
-
-      assert BC.Freeze(Ik(k), IVars(s), IVars(s'), ImplADM.IDiskOp(io.diskOp()));
-      assert BBC.BlockCacheMove(Ik(k), IVars(s), IVars(s'), UI.NoOp, ImplADM.IDiskOp(io.diskOp()), BC.FreezeStep);
+      assert BC.Freeze(Ik(k), IVars(s), IVars(s'), M.IDiskOp(diskOp(io')));
+      assert BBC.BlockCacheMove(Ik(k), IVars(s), IVars(s'), UI.NoOp, M.IDiskOp(diskOp(io')), BC.FreezeStep);
       assert stepsBC(k, IVars(s), IVars(s'), UI.NoOp, io, BC.FreezeStep);
       return;
     }
   }
 
-  method {:fuel BC.GraphClosed,0} syncFoundInFrozen(k: Constants, s: Variables, io: IO, ref: Reference)
-  returns (s': Variables)
-  requires io.initialized()
-  modifies io
-  requires WFVars(s)
-  requires BBC.Inv(k, IVars(s))
+  predicate {:fuel BC.GraphClosed,0} syncFoundInFrozen(k: Constants, s: Variables, io: IO, ref: Reference,
+      s': Variables, io': IO)
+  requires io.IOInit?
+  requires Inv(k, s)
   requires s.Ready?
   requires s.outstandingIndirectionTableWrite.None?
-  requires s.rootBucket == TTT.EmptyTree
+  requires s.rootBucket == map[]
   requires s.frozenIndirectionTable.Some?
-  requires ref in IIndirectionTable(s.frozenIndirectionTable.value).graph 
-  requires ref !in IIndirectionTable(s.frozenIndirectionTable.value).locs
-  ensures WFVars(s')
-  ensures ImplADM.Next(Ik(k), IVars(s), IVars(s'), UI.NoOp, io.diskOp())
+  requires ref in s.frozenIndirectionTable.value
+  requires s.frozenIndirectionTable.value[ref].0.None?
   {
     assert ref in IIndirectionTable(s.frozenIndirectionTable.value).graph;
     assert ref !in IIndirectionTable(s.frozenIndirectionTable.value).locs;
 
-    if (!Marshalling.CappedNode(s.cache[ref])) {
+    if (!IMM.CappedNode(s.cache[ref])) then (
       // TODO we should be able to prove this is impossible by adding an invariant
       // about frozenIndirectionTable (that is, we should never be freezing a table
       // with too-big nodes in it)
-      s' := s;
-      assert noop(k, IVars(s), IVars(s'));
-      print "sync: giving up; frozen table has big node rip (TODO we should prove this case impossible)\n";
+      && s' == s
+      && io' == io
+    ) else (
+      if ref in s.ephemeralIndirectionTable && s.ephemeralIndirectionTable[ref].0.Some? then (
+        // TODO we should be able to prove this is impossible as well
+        && s' == s
+        && io' == io
+      ) else (
+        if diskOp(io').ReqWriteOp? && s'.Ready? && ref in s'.ephemeralIndirectionTable && s'.ephemeralIndirectionTable[ref].0.Some? then (
+          var id := Some(diskOp(io').id);
+          var loc := s'.ephemeralIndirectionTable[ref].0;
+          && FindLocationAndRequestWrite(io, s, SectorBlock(s.cache[ref]), id, loc, io')
+
+          && s' == s
+            .(outstandingBlockWrites := s.outstandingBlockWrites[id.value := BC.OutstandingWrite(ref, loc.value)])
+            .(ephemeralIndirectionTable := AssignRefToLoc(s.ephemeralIndirectionTable, ref, loc.value))
+            .(frozenIndirectionTable := Some(AssignRefToLoc(s.frozenIndirectionTable.value, ref, loc.value)))
+        ) else (
+          && s' == s
+          && io' == io
+        )
+      )
+    )
+  }
+
+  lemma {:fuel BC.GraphClosed,0} syncFoundInFrozenCorrect(k: Constants, s: Variables, io: IO, ref: Reference,
+      s': Variables, io': IO)
+  requires io.IOInit?
+  requires Inv(k, s)
+  requires s.Ready?
+  requires s.outstandingIndirectionTableWrite.None?
+  requires s.rootBucket == map[]
+  requires s.frozenIndirectionTable.Some?
+  requires ref in s.frozenIndirectionTable.value
+  requires s.frozenIndirectionTable.value[ref].0.None?
+
+  requires syncFoundInFrozen(k, s, io, ref, s', io')
+
+  ensures WFVars(s')
+  ensures M.Next(Ik(k), IVars(s), IVars(s'), UI.NoOp, diskOp(io'))
+  {
+    assert ref in IIndirectionTable(s.frozenIndirectionTable.value).graph;
+    assert ref !in IIndirectionTable(s.frozenIndirectionTable.value).locs;
+
+    if (!IMM.CappedNode(s.cache[ref])) {
+      assert noop(k, IVars(s), IVars(s));
       return;
     }
 
-    var ephemeralRef := s.ephemeralIndirectionTable.Get(ref);
-    if ephemeralRef.Some? && ephemeralRef.value.0.Some? {
+    if ref in s.ephemeralIndirectionTable && s.ephemeralIndirectionTable[ref].0.Some? {
       assert ref in IIndirectionTable(s.ephemeralIndirectionTable).locs;
-      // TODO we should be able to prove this is impossible as well
-      s' := s;
-      assert noop(k, IVars(s), IVars(s'));
-      print "sync: giving up; ref already in ephemeralIndirectionTable.locs but not frozen";
+      assert noop(k, IVars(s), IVars(s));
       return;
     }
 
     assert ref !in IIndirectionTable(s.ephemeralIndirectionTable).locs;
 
     INodeRootEqINodeForEmptyRootBucket(s.cache[ref]);
-    var id, loc := FindLocationAndRequestWrite(s, io, SectorBlock(s.cache[ref]));
-    if (id.Some?) {
-      assert loc.value == ImplADM.IDiskOp(io.diskOp()).reqWrite.loc;
-      /* (doc) assert reqWriteLoc.addr != BC.IndirectionTableLBA(); */
-      /* (doc) assert BC.ValidAllocation(IVars(s), loc.value); */
 
-      AssignRefToLBA(s.ephemeralIndirectionTable, ref, loc.value);
-      assert IIndirectionTable(s.ephemeralIndirectionTable) ==
-        BC.assignRefToLocation(IIndirectionTable(s.ephemeralIndirectionTable), ref, loc.value);
-      AssignRefToLBA(s.frozenIndirectionTable.value, ref, loc.value);
-      assert IIndirectionTable(s.frozenIndirectionTable.value) ==
-        BC.assignRefToLocation(IIndirectionTable(s.frozenIndirectionTable.value), ref, loc.value);
-      s' := s
-        .(outstandingBlockWrites := s.outstandingBlockWrites[id.value := BC.OutstandingWrite(ref, loc.value)]);
+    if diskOp(io').ReqWriteOp? && s'.Ready? && ref in s'.ephemeralIndirectionTable && s'.ephemeralIndirectionTable[ref].0.Some? {
+      var id := Some(diskOp(io').id);
+      var loc := s'.ephemeralIndirectionTable[ref].0;
+      FindLocationAndRequestWriteCorrect(io, s, SectorBlock(s.cache[ref]), id, loc, io');
 
-      assert BC.ValidLocationForNode(ImplADM.IDiskOp(io.diskOp()).reqWrite.loc);
-      assert BC.WriteBackReq(Ik(k), IVars(s), IVars(s'), ImplADM.IDiskOp(io.diskOp()), ref);
-      assert stepsBC(k, IVars(s), IVars(s'), UI.NoOp, io, BC.WriteBackReqStep(ref));
-      return;
+      AssignRefToLocCorrect(s.ephemeralIndirectionTable, ref, loc.value);
+      AssignRefToLocCorrect(s.frozenIndirectionTable.value, ref, loc.value);
+
+      assert BC.ValidLocationForNode(M.IDiskOp(diskOp(io')).reqWrite.loc);
+      assert BC.WriteBackReq(Ik(k), IVars(s), IVars(s'), M.IDiskOp(diskOp(io')), ref);
+      assert stepsBC(k, IVars(s), IVars(s'), UI.NoOp, io', BC.WriteBackReqStep(ref));
     } else {
-      s' := s;
-      assert noop(k, IVars(s), IVars(s'));
-      print "sync: giving up; write req failed\n";
-      return;
+      assert noop(k, IVars(s), IVars(s));
     }
   }
+
+
+
+  /*
 
   method {:fuel BC.GraphClosed,0} sync(k: Constants, s: Variables, io: IO)
   returns (s': Variables)
@@ -435,7 +424,7 @@ module ImplModelSync {
   requires WFVars(s)
   requires BBC.Inv(k, IVars(s))
   ensures WFVars(s')
-  ensures ImplADM.Next(Ik(k), IVars(s), IVars(s'), UI.NoOp, io.diskOp())
+  ensures Next(Ik(k), IVars(s), IVars(s'), UI.NoOp, io.diskOp())
   {
     if (s.Unready?) {
       // TODO we could just do nothing here instead
@@ -482,7 +471,7 @@ module ImplModelSync {
       var id := RequestWrite(io, BC.IndirectionTableLocation(), SectorIndirectionTable(s.frozenIndirectionTable.value));
       if (id.Some?) {
         s' := s.(outstandingIndirectionTableWrite := id);
-        assert BC.WriteBackIndirectionTableReq(Ik(k), IVars(s), IVars(s'), ImplADM.IDiskOp(io.diskOp()));
+        assert BC.WriteBackIndirectionTableReq(Ik(k), IVars(s), IVars(s'), M.IDiskOp(io.diskOp()));
         assert stepsBC(k, IVars(s), IVars(s'), UI.NoOp, io, BC.WriteBackIndirectionTableReqStep);
         return;
       } else {
@@ -514,7 +503,7 @@ module ImplModelSync {
   requires WFVars(s)
   requires BBC.Inv(k, IVars(s))
   ensures WFVars(s')
-  ensures ImplADM.Next(Ik(k), IVars(s), IVars(s'), UI.PushSyncOp(id), io.diskOp())
+  ensures M.Next(Ik(k), IVars(s), IVars(s'), UI.PushSyncOp(id), io.diskOp())
   {
     id := freeId(s.syncReqs);
     s' := s.(syncReqs := s.syncReqs[id := BC.State3]);
@@ -530,7 +519,7 @@ module ImplModelSync {
   requires BBC.Inv(k, IVars(s))
   modifies io
   ensures WFVars(s')
-  ensures ImplADM.Next(Ik(k), IVars(s), IVars(s'), if success then UI.PopSyncOp(id) else UI.NoOp, io.diskOp())
+  ensures M.Next(Ik(k), IVars(s), IVars(s'), if success then UI.PopSyncOp(id) else UI.NoOp, io.diskOp())
   {
     if (id in s.syncReqs && s.syncReqs[id] == BC.State1) {
       success := true;
